Added more verification to the BubbleSort, regarding permutations

verification/BubbleSort.dfy
@@ -1,8 +1,54 @@
+// Recursively count the number of appearances 'k' has in sequence 'a'
+function count(a: seq<int>, k: int): nat{
+  if |a| == 0 then 0 else (if a[0] == k then 1 else 0) + count(a[1..],k)
+}
+
+/*
+  Counting the instances of a key in the sum of two sequences,
+  is the same as summing the instances of the key in each sequence
+*/
+lemma distributiveCount(a: seq<int>, b: seq<int>)
+ensures forall k:: count(a + b,k) == count(a,k) + count(b,k)
+{
+  if (|a| == 0){
+    assert a + b == b;
+  } else {
+    distributiveCount(a[1..],b);
+    assert a == [a[0]] + a[1..];
+    assert a + b == [a[0]] + (a[1..] + b);
+  }
+}
+
+/*
+  If we have two pairs of seq's that are permutations of each other, then
+  it must be true that their sums are also permutations.
+*/
+lemma distributivePerm(a: seq<int>,a': seq<int>,b: seq<int>,b': seq<int>)
+requires PermOf(a,a')
+requires PermOf(b,b')
+ensures PermOf(a+b,a'+b')
+{
+  assert forall i:: count(a,i) == count(a',i);
+  assert forall i:: count(b,i) == count(b',i);
+  assert forall k:: count(a,k) + count(b,k) == count(a',k) + count(b',k);
+  distributiveCount(a,b);
+  distributiveCount(a',b');
+  assert forall k:: count(a + b,k) == count(a,k) + count(b,k);
+  assert forall k:: count(a' + b',k) == count(a',k) + count(b',k);
+  assert PermOf(a+b,a'+b');
+}
+
+// Check if one sequence is a permutation of another by counting appearances of keys
+predicate PermOf(a: seq<int>, b: seq<int>) {
+  forall i: int :: count(a,i) == count(b,i)
+}
+
 // Check is a[x..] is sorted
 predicate Sorted(a: seq<int>, x: int)
 {
     forall i, j :: 0 <= x <= i <= j < |a| ==> a[i] <= a[j]
 }
+
 /*
     Checks if the right portion of a partition split at index i
     is greater than the left portion
@@ -13,42 +59,76 @@ predicate Less(a: seq<int>, i: int)
 }
 
 method BubbleSort(a: array<int>)
-    requires a != null
-    modifies a
-    ensures Sorted(a[..], 0)
+modifies a;
+ensures Less(a[..],0)
+ensures Sorted(a[..],0)
+ensures PermOf(old (a[..]), a[..])
 {
-    if a.Length == 0 { return; }
-    var i := a.Length - 1;
-    while i > 0
-    invariant 0 <= i < a.Length
-    // a[i..] is sorted and a[..i] <= a[i..]
-    invariant Sorted(a[..], i) && Less(a[..], i)
-    /*
-        i.e. since a[..i] shrinks to 0, ensuring [1] & [2] will ensure that
-        a[i..] is always sorted. As i eventually decreases to 0, the result
-        will be that a[0..] is sorted, i.e. the entire array is sorted
-    */
+  if a.Length == 0 { return; }
+  var i := a.Length - 1;
+  while (i > 0)
+  invariant 0 <= i < a.Length
+  invariant Less(a[..],i)
+  invariant Sorted(a[..], i)
+  // a[i..] is sorted and a[..i] <= a[i..]
+  invariant PermOf(old (a[..]), a[..])
+  /*
+      i.e. since a[..i] shrinks to 0, ensuring [1] & [2] will ensure that
+      a[i..] is always sorted. As i eventually decreases to 0, the result
+      will be that a[0..] is sorted, i.e. the entire array is sorted
+  */
+  {
+    var j := 0;
+    while (j < i)
+    invariant 0 <= j <= i
+    invariant forall k:: 0 <= k < j ==> a[k] <= a[j]  // a[..j] <= a[j]
+    invariant Sorted(a[..],i)                         // a[i..] is sorted
+    invariant Less(a[..],i)                           // a[..i] <= a[i..]
+    invariant PermOf(old (a[..]), a[..])              // Current array is a perm. of the original array
     {
-        var j := 0;
-        while j < i
-        invariant 0 <= j <= i
-        // a[i..] is sorted and a[..i] <= a[i..]
-        invariant Sorted(a[..], i) && Less(a[..], i)
-        // a[..j] <= a[j]
-        invariant forall k :: 0 <= k < j ==> a[k] <= a[j]
-        {
-            if a[j] > a[j + 1] { a[j], a[j + 1] := a[j + 1], a[j]; }
-            j := j + 1;
-        }
-        i := i - 1;
+      ghost var a' := a[..];                          // Save instance of array before any swapping
+      ghost var v1,v2 := a[j],a[j+1];                 // Get the two variables that (may) be swapped
+//      assert a[..] == a[0..j] + [v1,v2] + a[j+2..];
+      
+      if (a[j] > a[j + 1]){                           // Swap if necessary
+        a[j],a[j+1] := a[j+1],a[j];
+      }
+      
+      /*
+        Intution for the proof:
+          We may partition the seq 'a' into 3 subsets: a[..i],a[i,i+1],a[i+2..].
+          Clearly, these subsets are disjoint and their sum is 'a'.
+          During the swap, these subsets are individually permuted within themselves,
+            that is, no member of a subset will end up in a different subset after the swap.
+          We formalise this by saying that a[..i],a[i,i+1],a[i+2..] are each unaffected up to a permutation
+          We assert these individually, and also use the distributive lemma regarding permutations
+            to show that therefore the whole array is a permutation of the original array
+      */
+      
+      ghost var v3,v4 := a[j],a[j+1];                     // Save two variables that (may) have been swapped
+      assert PermOf([v1,v2],[v3,v4]);
+      assert PermOf(a'[0..j],a[0..j]);
+      distributivePerm(a'[0..j],a[0..j],[v1,v2],[v3,v4]);
+      
+      assert PermOf(a'[0..j] + [v1,v2],a[0..j] + [v3,v4]);
+      assert PermOf(a'[j+2..],a[j+2..]);
+      distributivePerm(a'[0..j]+[v1,v2],a[0..j]+[v3,v4],a'[j+2..],a[j+2..]);
+      
+      assert a'[..] == a'[0..j] + [v1,v2] + a'[j+2..];
+      assert a[..] == a[0..j] + [v3,v4] + a[j+2..];
+      assert PermOf(a',a[..]);
+      
+      j := j + 1;
     }
+    i := i - 1;
+  }
 }
+
 
 method Main() {
     var a := new int[5];
     a[0], a[1], a[2], a[3], a[4] := 9, 4, 6, 3, 8;
     BubbleSort(a);
-    assert Sorted(a[..], 0);
     var b := new int[0];
     BubbleSort(b);
     assert Sorted(b[..], 0);
